@prefix rdf: <http://www.w3.org/1999/02/22-rdf-syntax-ns#> .
@prefix rdfs: <http://www.w3.org/2000/01/rdf-schema#> .
@prefix owl: <http://www.w3.org/2002/07/owl#> .
@prefix skos: <http://www.w3.org/2004/02/skos/core#> .


<http://example.org/openWEMI/> a owl:Ontology ;
  rdfs:label "openWEMI ontology" ;
  rdfs:comment "The openWEMI ontology provides a high-level skeleton for vocabularies to build on. Like owl:Thing, the classes are so broad that it is expected that vocabularies describing types of creations will subclass to the openWEMI classes in a way to better describes their targets. The same is true of the properties provided in openWEMI. There are no restrictions on using openWEMI with additional classes or properties. openWEMI builds on the work done in the library community (FRBR) but with many fewer constraints, thus making reuse easier."@en .

<http://example.org/openWEMI/Endeavor>
  a owl:Class ;
  rdfs:label "endeavour"@en ;
  skos:definition "A creation."@en ;
  rdfs:isDefinedBy <http://example.org/openWEMI/> ;
  rdfs:comment "Endeavor is an umbrella class that unites the classes Work, Expression, Manifestation, Item."@en .
  
<http://example.org/openWEMI/Work>
  a owl:Class ;
  rdfs:label "work"@en ;
  skos:definition "An abstract notion of an artistic or intellectual creation."@en ;
  rdfs:isDefinedBy <http://example.org/openWEMI/> ;
  rdfs:subClassOf <http://example.org/openWEMI/Endeavor> ;
  rdfs:comment "Each metadata community will have a different definition of Work, but it should be the broadest definition of the creations being described. A work is an abstraction that represents the concepts behind a creation."@en .
  
<http://example.org/openWEMI/Expression>
  a owl:Class ;
  rdfs:label "expression"@en ;
  skos:definition "A perceivable form of the creation."@en ;
  rdfs:isDefinedBy <http://example.org/openWEMI/> ;
  rdfs:subClassOf <http://example.org/openWEMI/Endeavor> ;
  rdfs:comment "Creations are made tangible through some kind of expression, such as text, sound, or a visual form. There may be more than one expression of a work of the same type or of different types."@en .

<http://example.org/openWEMI/Manifestation>
  a owl:Class ;
  rdfs:label "manifestation"@en ;
  skos:definition "The physical embodiment of a creation."@en ;
  rdfs:isDefinedBy <http://example.org/openWEMI/> ;
  rdfs:subClassOf <http://example.org/openWEMI/Endeavor> ;
  rdfs:comment "A manifestation is a creation that has been realized in some physical or digital form. A manifestation may be a single realization or a realization that is produced in multiple copies such as the publication of a music compact disk or the manufacture of a shirt."@en .
  
<http://example.org/openWEMI/Item>
  a owl:Class ;
  rdfs:label "item"@en ;
  skos:definition "An exemplar of a creation."@en ;
  rdfs:isDefinedBy <http://example.org/openWEMI/> ;
  rdfs:subClassOf <http://example.org/openWEMI/Endeavor> ;
  rdfs:comment "An item is a single instance of the creation, something that can have a place on a shelf or a location online."@en .

<http://example.org/openWEMI/responsibleEntity>
  a rdfs:Property ;
  rdfs:label "responsible entity"@en ;
  skos:definition "One responsible for the creation, production, distribution, maintenance, or ownership of a created entity."@en ;
  rdfs:isDefinedBy <http://example.org/openWEMI/> ;
  rdfs:domain <http://example.org/openWEMI/Endeavor> ;
  rdfs:comment "It is assumed that creations have been affected by an agent with the ability to act. The types of agents is very broad and not constrained by this property."@en .
      
<http://example.org/openWEMI/relatedEndeavor>
  a rdfs:Property ;
  rdfs:label "related endeavor"@en ;
  skos:definition "Another endeavor that is related in some way to an endeavor."@en ;
  rdfs:isDefinedBy <http://example.org/openWEMI/> ;
  rdfs:domain <http://example.org/openWEMI/Endeavor> ;
  rdfs:range <http://example.org/openWEMI/Endeavor> ;
  rdfs:comment "This provides a non-specific relationship between two endeavors. The relationship type can be defined as a sub-property of relatedEndeavor."@en .

<http://example.org/openWEMI/relatedWork>
  a rdfs:Property ;
  rdfs:label "related work"@en ;
  skos:definition "Another work that is related in some way to a work."@en ;
  rdfs:isDefinedBy <http://example.org/openWEMI/> ;
  rdfs:domain <http://example.org/openWEMI/Work> ;
  rdfs:range <http://example.org/openWEMI/Work> ;
  rdfs:comment "This provides a non-specific relationship between two works. The relationship type can be defined as a sub-property of relatedWork."@en

<http://example.org/openWEMI/relatedExpression>
  a rdfs:Property ;
  rdfs:label "related expression"@en ;
  skos:definition "Another expression that is related in some way to an expression."@en ;
  rdfs:isDefinedBy <http://example.org/openWEMI/> ;
  rdfs:domain <http://example.org/openWEMI/Expression> ;
  rdfs:range <http://example.org/openWEMI/Expression> ;
  rdfs:comment "This provides a non-specific relationship between two expressions. The relationship type can be defined as a sub-property of relatedExpression."@en .

<http://example.org/openWEMI/relatedManifestation>
  a rdfs:Property ;
  rdfs:label "related manifestation"@en ;
  skos:definition "Another manifestation that is related in some way to a manifestation."@en ;
  rdfs:isDefinedBy <http://example.org/openWEMI/> ;
  rdfs:domain <http://example.org/openWEMI/Manifestation> ;
  rdfs:range <http://example.org/openWEMI/Manifestation> ;
  rdfs:comment "This provides a non-specific relationship between two manifestations. The relationship type can be defined as a sub-property of relatedManifestation."@en .

<http://example.org/openWEMI/relatedItem>
  a rdfs:Property ;
  rdfs:label "related item"@en ;
  skos:definition "Another item that is related in some way to an item."@en ;
  rdfs:isDefinedBy <http://example.org/openWEMI/> ;
  rdfs:domain <http://example.org/openWEMI/Item> ;
  rdfs:range <http://example.org/openWEMI/Item> ;
  rdfs:comment "This provides a non-specific relationship between two items. The relationship type can be defined as a sub-property of relatedItem."@en .

<http://example.org/openWEMI/expresses>
  a rdfs:Property ;
  rdfs:label "expresses"@en ;
  skos:definition "An endeavor that expresses a work."@en ;
  rdfs:isDefinedBy <http://example.org/openWEMI/> ;
  rdfs:subPropertyOf <http://example.org/openWEMI/relatedEndeavor> ;
  rdfs:domain <http://example.org/openWEMI/Expression> ;
  rdfs:range <http://example.org/openWEMI/Work> ;
  rdfs:comment "A relationship asserted from an Expression to a Work; the expression of the Work."@en .


 <http://example.org/openWEMI/expressedBy>
  a rdfs:Property ;
  rdfs:label "expressed by"@en ;
  skos:definition "An expression of a work."@en ;
  owl:inverseOf <http://example.org/openWEMI/expresses> ;
  rdfs:isDefinedBy <http://example.org/openWEMI/> ;
  rdfs:subPropertyOf <http://example.org/openWEMI/relatedEndeavor> ;
  rdfs:domain <http://example.org/openWEMI/Work> ;
  rdfs:range <http://example.org/openWEMI/Expression> ; 
  rdfs:comment "A relationship asserted from a Work to an Expression; an Expression that expresses the Work."@en .


<http://example.org/openWEMI/manifests>
  a rdfs:Property ;
  rdfs:label "manifests"@en ;
  skos:definition "An endeavor that manifests an expression or a work."@en ;
  rdfs:isDefinedBy <http://example.org/openWEMI/> ;
  rdfs:subPropertyOf <http://example.org/openWEMI/relatedEndeavor> ;
  rdfs:domain <http://example.org/openWEMI/Manifestation> ;
  rdfs:range [
    a owl:Class ;
    owl:unionOf (
      <http://example.org/openWEMI/Work> 
      <http://example.org/openWEMI/Expression>
    )
  ] .

<http://example.org/openWEMI/manifestedBy>
  a rdfs:Property ;
  rdfs:label "manifested by"@en ;
  skos:definition "A manifestation of a work or an expression."@en ;
  owl:inverseOf <http://example.org/openWEMI/manifests> ;
  rdfs:isDefinedBy <http://example.org/openWEMI/> ;
  rdfs:subPropertyOf <http://example.org/openWEMI/relatedEndeavor> ;
  rdfs:domain [
      a owl:Class ;
      owl:unionOf (
       <http://example.org/openWEMI/Work> 
       <http://example.org/openWEMI/Expression>
     )
    ] ;
  rdfs:range <http://example.org/openWEMI/Manifestation> . 

    
<http://example.org/openWEMI/instantiates>
  a rdfs:Property ;
  rdfs:label "instantiates"@en ;
  skos:definition "An endeavor that instantiates a manifestation, an expression or a work."@en ;
  rdfs:isDefinedBy <http://example.org/openWEMI/> ;
  rdfs:subPropertyOf <http://example.org/openWEMI/relatedEndeavor> ;
  rdfs:domain <http://example.org/openWEMI/Item> ;
  rdfs:range [
    a owl:Class ;
    owl:unionOf (
      <http://example.org/openWEMI/Work>
      <http://example.org/openWEMI/Expression>
      <http://example.org/openWEMI/Manifestation>
    )
  ] .


<http://example.org/openWEMI/instantiatedBy>
  a rdfs:Property ;
  rdfs:label "instantiated by"@en ;
  skos:definition "An instatiation of a manifestation, an expression or a work."@en ;
  owl:inverseOf <http://example.org/openWEMI/instantiates> ;
  rdfs:isDefinedBy <http://example.org/openWEMI/> ;
  rdfs:subPropertyOf <http://example.org/openWEMI/relatedEndeavor> ;
  rdfs:domain [
      a owl:Class ;
      owl:unionOf (
       <http://example.org/openWEMI/Work> 
       <http://example.org/openWEMI/Expression>
       <http://example.org/openWEMI/Manifestation>
     )
    ] ;
  rdfs:range <http://example.org/openWEMI/Item> . 

